pulse/share/steel/examples/pulse/dice/dpe/DPE.Messages.Parse.fst
@@ -111,8 +111,8 @@ let parse_dpe_cmd_post
 = match res with
   | None -> A.pts_to input #p s ** pure (parse_dpe_cmd_failure_postcond s)
   | Some cmd -> exists_ (fun vargs ->
-      raw_data_item_match cmd.dpe_cmd_args vargs **
-      (raw_data_item_match cmd.dpe_cmd_args vargs @==>
+      raw_data_item_match full_perm cmd.dpe_cmd_args vargs **
+      (raw_data_item_match full_perm cmd.dpe_cmd_args vargs @==>
         A.pts_to input #p s
       ) **
       pure (
@@ -145,10 +145,10 @@ fn parse_dpe_cmd (len:SZ.t)
       ParseSuccess c ->
       {
         unfold (read_deterministically_encoded_cbor_with_typ_post Spec.session_message input p s (ParseSuccess c));
-        with vc . assert (raw_data_item_match c.read_cbor_payload vc);
+        with vc . assert (raw_data_item_match full_perm c.read_cbor_payload vc);
         with vrem1 . assert (A.pts_to c.read_cbor_remainder #p vrem1);
         stick_consume_r ()
-          #(raw_data_item_match c.read_cbor_payload vc)
+          #(raw_data_item_match full_perm c.read_cbor_payload vc)
           #(A.pts_to c.read_cbor_remainder #p vrem1)
           #(A.pts_to input #p s)
         ;
@@ -160,13 +160,13 @@ fn parse_dpe_cmd (len:SZ.t)
         stick_trans ();
         let cbor_str = destr_cbor_string i1;
         stick_trans ();
-        with cs . assert (A.pts_to cbor_str.cbor_string_payload #cbor_str.permission cs);
+        with cs ps . assert (A.pts_to cbor_str.cbor_string_payload #ps cs);
         let msg_rc = read_deterministically_encoded_cbor_with_typ impl_command_message' cbor_str.cbor_string_payload (SZ.of_u64 cbor_str.cbor_string_length);
         match msg_rc
         {
           ParseError ->
           {
-            unfold (read_deterministically_encoded_cbor_with_typ_post Spec.command_message' cbor_str.cbor_string_payload cbor_str.permission cs ParseError);
+            unfold (read_deterministically_encoded_cbor_with_typ_post Spec.command_message' cbor_str.cbor_string_payload ps cs ParseError);
             elim_implies ();
             serialize_cbor_inj' vc vrem1;
             fold (parse_dpe_cmd_post len input s p None);
@@ -174,13 +174,13 @@ fn parse_dpe_cmd (len:SZ.t)
           }
           ParseSuccess msg ->
           {
-            unfold (read_deterministically_encoded_cbor_with_typ_post Spec.command_message' cbor_str.cbor_string_payload cbor_str.permission cs (ParseSuccess msg));
-            with vmsg . assert (raw_data_item_match msg.read_cbor_payload vmsg);
-            with vrem2 . assert (A.pts_to msg.read_cbor_remainder #cbor_str.permission vrem2);
+            unfold (read_deterministically_encoded_cbor_with_typ_post Spec.command_message' cbor_str.cbor_string_payload ps cs (ParseSuccess msg));
+            with vmsg . assert (raw_data_item_match full_perm msg.read_cbor_payload vmsg);
+            with vrem2 . assert (A.pts_to msg.read_cbor_remainder #ps vrem2);
             stick_consume_r ()
-              #(raw_data_item_match msg.read_cbor_payload vmsg)
-              #(A.pts_to msg.read_cbor_remainder #cbor_str.permission vrem2)
-              #(A.pts_to cbor_str.cbor_string_payload #cbor_str.permission cs)
+              #(raw_data_item_match full_perm msg.read_cbor_payload vmsg)
+              #(A.pts_to msg.read_cbor_remainder #ps vrem2)
+              #(A.pts_to cbor_str.cbor_string_payload #ps cs)
             ;
             stick_trans ();
             if (msg.read_cbor_remainder_length <> 0sz) {
@@ -196,7 +196,7 @@ fn parse_dpe_cmd (len:SZ.t)
               elim_implies ();
               let cmd_args = cbor_array_index msg.read_cbor_payload 1sz;
               stick_trans ();
-              with vargs . assert (raw_data_item_match cmd_args vargs);
+              with vargs . assert (raw_data_item_match full_perm cmd_args vargs);
 
               let res = Mkdpe_cmd sid cmd_id cmd_args;
 (*  // FIXME: WHY WHY WHY does the following record literal FAIL with "List.combine: list lengths differ"
@@ -205,8 +205,8 @@ fn parse_dpe_cmd (len:SZ.t)
                 dpe_cmd_args = cmd_args;
               };
 *)              
-              rewrite (raw_data_item_match cmd_args vargs ** `@(raw_data_item_match cmd_args vargs @==> A.pts_to input #p s)) // FIXME: should `fold` honor projectors and not just `match`?
-                as (raw_data_item_match res.dpe_cmd_args vargs ** `@(raw_data_item_match res.dpe_cmd_args vargs @==> A.pts_to input #p s));
+              rewrite (raw_data_item_match full_perm cmd_args vargs ** `@(raw_data_item_match full_perm cmd_args vargs @==> A.pts_to input #p s)) // FIXME: should `fold` honor projectors and not just `match`?
+                as (raw_data_item_match full_perm res.dpe_cmd_args vargs ** `@(raw_data_item_match full_perm res.dpe_cmd_args vargs @==> A.pts_to input #p s));
               fold (parse_dpe_cmd_post len input s p (Some res));
               Some res
             }
